Attempt at infinite paths

Ctl/Paths.v
@@ -29,14 +29,14 @@ CoInductive forall_in_path {state R s} (P: state -> Prop) : path R s -> Prop :=
       @forall_in_path state R s' P p ->
       forall_in_path P (step s s' r p).
 
-Inductive in_path {state: Type} {R: relation state} {s} : state -> path R s -> Prop :=
+Inductive in_path {state} {R: relation state} {s} : state -> path R s -> Prop :=
   | in_head : forall s' r p,
       in_path s (step s s' r p)
   | in_tail : forall s' x r p,
       @in_path state R s' x p ->
       in_path x (step s s' r p).
 
-Definition forall_in_path' {state: Type} {R: relation state} {s: state}
+Definition forall_in_path' {state} {R: relation state} {s: state}
   (P: state -> Prop) (p: path R s) :=
   forall s', in_path s' p -> P s'.
 
@@ -52,7 +52,7 @@ CoInductive exists_path {state R} (P: state -> Prop) (s: state) : Prop :=
       exists_path P s.
 
 (* Require Import Coq.Vectors.VectorDef. *)
-Inductive finite_path {state} (R: relation state) : state -> nat -> Prop := 
+Inductive finite_path {state} (R: relation state) : state -> nat -> Type := 
   | finite_trivial : forall s, finite_path R s 0
   | finite_step : forall s s' n,
       R s s' ->
@@ -79,7 +79,55 @@ Fixpoint path_to_finite {state} {R: relation state} {s}
       end
   end.
 
-Lemma in_path_refl_finite {state} {R: relation state} {s} :
+Require Import Psatz.
+Definition finite_path_pop n {state} {R: relation state} {m s} (fp: finite_path R s m) 
+  : {s' & finite_path R s' (m-n)}.
+  induction n.
+  - exists s.
+    replace (m - 0) with m by lia.
+    assumption.
+  - destructExists IHn s'.
+    inv IHn.
+    + exists s'.
+      rewrite <- H1 in IHn.
+      replace (m - S n) with 0 by lia.
+      assumption.
+    + exists s'0.
+      replace (m - S n) with n0 by lia.
+      assumption.
+Qed.
+
+Definition finite_path_tail {state} {R: relation state} {s n}
+  (fp: finite_path R s (S n)) : {s' & finite_path R s' n}.
+inv fp.
+eexists.
+eassumption.
+Defined.
+
+Lemma finite_path_tail_correct {state} {R: relation state}:
+  forall s s' n r (fp: finite_path R s' n),
+  (* finite_path_tail (finite_step s s' n r fp) = existT _ s' fp. *)
+  projT2 (finite_path_tail (finite_step s s' n r fp)) = fp.
+Proof. reflexivity. Qed.
+
+Definition finite_path_get_step {state} {R: relation state} {m s}
+  n (HinBounds: n < m) (fp: finite_path R s m) : {x & {y | R x y}}.
+max_induction n; intros.
+- inv fp.
+  + lia.
+  + repeat eexists. eassumption.
+- destruct m as [|m']; [lia|].
+  inv fp.
+  clear H1.
+  assert (HLt: n < m') by lia.
+  specialize (IHn state R m' s' HLt X).
+  destructExists IHn x.
+  destructExists IHn y.
+  repeat eexists.
+  eapply IHn.
+Defined.
+
+Theorem in_path_refl_finite {state} {R: relation state} {s} :
   forall (p: path R s) s',
   in_path s' p ->
   exists n, in_finite_path s' n (path_to_finite p n).
@@ -92,6 +140,28 @@ Proof.
     exists (S n).
     constructor; assumption.
 Qed.
+
+Theorem in_path_refl_infinite {state} {R: relation state} {s} :
+  forall (p: path R s) s',
+  (exists n, in_finite_path s' n (path_to_finite p n)) ->
+  in_path s' p.
+Proof.
+  (* intros p. *)
+
+  intros p s' H.
+  destructExists H n.
+  induction H.
+  - destruct p; constructor.
+  - 
+  
+Admitted.
+
+Theorem in_path_refl {state} {R: relation state} {s} :
+  forall (p: path R s) s',
+  in_path s' p <->
+  exists n, in_finite_path s' n (path_to_finite p n).
+Proof.
+Admitted.
 
 Theorem forall_in_path_refl_finite {state} {R: relation state} {s}:
   forall (P: state -> Prop) (p: path R s),
@@ -108,9 +178,20 @@ Proof.
     constructor; assumption.
 Qed.
 
+Require Import Coq.Program.Equality.
 Theorem exists_in_path_refl_finite {state} {R: relation state} {s}:
   forall P (p: path R s),
     (exists n s', in_finite_path s' n (path_to_finite p n) /\ P s') ->
     (exists s', in_path s' p /\ P s').
 Proof.
+  intros P p H.
+  destruct H as [n [s' [Hin HP]]].
+  exists s'.
+  split; [|assumption].
+  dependent induction Hin.
+  - destruct p as [x' r' p].
+    simpl in x.
+    assert (s' = x'). { admit. }
+    constructor.
+  - try apply IHHin.
 Admitted.
